---
title: "Kernel density estimation"
output:
  pdf_document: default
  html_document: default
header-includes:
- \usepackage{color}
- \usepackage{graphicx}
- \usepackage{epic}
- \usepackage{hyperref}
- \PassOptionsToPackage{pdfmark}{hyperref}\RequirePackage{hyperref}
- \newcommand{\ve}[1]{\mathbf{#1}}
- \newcommand{\pop}[1]{\mathcal{#1}}
- \newcommand{\samp}[1]{\mathcal{#1}}
- \newcommand{\subspace}[1]{\mathcal{#1}}
- \newcommand{\sv}[1]{\boldsymbol{#1}}
- \newcommand{\sm}[1]{\boldsymbol{#1}}
- \newcommand{\tr}[1]{{#1}^{\mkern-1.5mu\mathsf{T}}}
- \newcommand{\abs}[1]{\left\lvert ~{#1} ~\right\rvert}
- \newcommand{\size}[1]{\left\lvert {#1} \right\rvert}
- \newcommand{\norm}[1]{\left|\left|{#1}\right|\right|}
- \newcommand{\field}[1]{\mathbb{#1}}
- \newcommand{\Reals}{\field{R}}
- \newcommand{\Integers}{\field{Z}}
- \newcommand{\Naturals}{\field{N}}
- \newcommand{\Complex}{\field{C}}
- \newcommand{\Rationals}{\field{Q}}
- \newcommand{\widebar}[1]{\overline{#1}}
- \newcommand{\wig}[1]{\tilde{#1}}
- \newcommand{\bigwig}[1]{\widetilde{#1}}
- \newcommand{\leftgiven}{~\left\lvert~}
- \newcommand{\given}{~\vert~}
- \newcommand{\indep}{\bot\hspace{-.6em}\bot}
- \newcommand{\notindep}{\bot\hspace{-.6em}\bot\hspace{-0.75em}/\hspace{.4em}}
- \newcommand{\depend}{\Join}
- \newcommand{\notdepend}{\Join\hspace{-0.9 em}/\hspace{.4em}}
- \newcommand{\imply}{\Longrightarrow}
- \newcommand{\notimply}{\Longrightarrow \hspace{-1.5em}/ \hspace{0.8em}}
- \newcommand*{\intersect}{\cap}
- \newcommand*{\union}{\cup}
- \newcommand{\suchthat}{~:~}
- \newcommand{\st}{~:~}
---

```{r setup, include=FALSE}
knitr::opts_chunk$set(echo = TRUE)
```

*Kernel density estimation.* 

a. Recall from the notes the general results on the bias (up to $O(h^4)$) and variance (up to order $O(\frac{h}{n})$) of a "simplified kernel" density estimator.

i. **(4 marks)** Prove that the following kernel is a ``simplified kernel'' (in the sense of the notes).

$$
\begin{aligned}
\int_{-1}^1K(w)dw &= \int_{-1}^1\frac{15}{32}(1-w^2)(3-7w^2)dw\\
&= \int_{-1}^1\frac{15}{32}(7w^4-10w^2+3)dw\\
&= \frac{15}{32}(\frac{7w^5}{5}-\frac{10w^3}{3}+3w)\rvert_{-1}^1\\
&= \frac{15}{32}[(\frac{7}{5}-\frac{10}{3}+3)-(\frac{-7}{5}+\frac{10}{3}-3)]\\
&= 1\\\\
\int_{-1}^1wK(w)dw &= \int_{-1}^1\frac{15}{32}w(1-w^2)(3-7w^2)dw\\
&= \int_{-1}^1\frac{15}{32}(7w^5-10w^3+3w)dw\\
&= \frac{15}{32}(\frac{7w^6}{6}-\frac{10w^4}{4}+\frac{3w^2}{2})\rvert_{-1}^1\\
&=\frac{15}{32}[(\frac{7}{6}-\frac{10}{4}+\frac{3}{2})-(\frac{7}{6}-\frac{10}{4}+\frac{3}{2})]\\
&= 0\\\\
\int_{-1}^1w^2K(w)dw &= \int_{-1}^1\frac{15}{32}w^2(1-w^2)(3-7w^2)dw\\
&= \int_{-1}^1\frac{15}{32}(7w^6-10w^4+3w^2)dw\\
&= \frac{15}{32}(\frac{7w^7}{7}-\frac{10w^5}{5}+\frac{3w^3}{3})\rvert_{-1}^1\\
&=   \frac{15}{32}(w^7-2w^5+w^3)\rvert_{-1}^1\\
&= \frac{15}{32}[(1-2+1)-(-1+2-1)]\\
&= 0 = \sigma_k^2\text{ } (0 \le \sigma_k^2 < \infty)\\
\\
&\text{Therefore, }K(w)\text{ is a simplified kernel.}
\end{aligned}
$$


ii. **(8 marks)** Determine the (approximate) mean squared error (from the slides) of $\tilde{f}_K(x)$ for the above kernel $K$ and for arbitrary $f(x)$.

$$
\begin{aligned}
Bias[\tilde{f}_k(x)]&=\frac{1}{2}\sigma_k^2h^2f''(x)+O(h^3)\\
&=0+O(h^3) \text{ } (as\text{ } \sigma_k^2=0)\\
&= O(h^3)\\\\
Var[\tilde{f}_k(x)]&=\frac{1}{nh}f(x)\int_{-1}^1{K^2(w)dw}-\frac{1}{n}[f(x)]^2+O(\frac{h^2}{n})\\
&=\frac{1}{nh}f(x)\frac{5}{4}-\frac{1}{n}[f(x)]^2+O(\frac{h^2}{n})\\
&=\frac{5}{4nh}-\frac{1}{n}[f(x)]^2+O(\frac{h^2}{n})\\\\
MSE &= Bias^2+Variance\\
&= Bias[\tilde{f}_k(x)]^2+Var[\tilde{f}_k(x)]\\
&= O(h^6) + \frac{5}{4nh}-\frac{1}{n}[f(x)]^2+O(\frac{h^2}{n})\\
&=\frac{5}{4nh}-\frac{1}{n}[f(x)]^2+O(h^6)\text{ Since }O(h^6)\text{ converges slower than }O(\frac{h^2}{n})
\end{aligned}
$$
    
iii. **(5 marks)** Determine the case for the above $K$ when the true underlying density $f(x)$ is $N(0,1)$.

$$
\begin{aligned}
f(x)&=\frac{1}{\sqrt{2\pi}}e^{\frac{-x^2}{2}}\\
MSE&=\frac{5}{4nh}-\frac{1}{n}[f(x)]^2+O(h^6)\\
&=\frac{5}{4nh}-\frac{1}{n}[\frac{1}{\sqrt{2\pi}}e^{\frac{-x^2}{2}}]^2+O(h^6)\\
&=\frac{5}{4nh}-\frac{1}{n}[\frac{1}{2\pi}e^{-x^2}]+O(h^6)\\
&=\frac{5}{4nh}-\frac{1}{2n\pi}e^{-x^2}+0(h^6)
\end{aligned}
$$